Wavelet/Dataflow/IndexedStep.lean
@@ -201,58 +201,19 @@ theorem Config.IndexedStep.unique_index
       inputs₂ inputVals₂ outputs₂ outputVals₂ _ hinterp₂ hpop₂ hget₂
     have ⟨h₁, h₂, h₃⟩ := hget₂
     subst h₁; subst h₂; subst h₃
-    have := async_op_interp_det_inputs_len hinterp₁ hinterp₂
-    simp at this
-    subst this
-    cases aop with
-    | merge =>
-      generalize hinputs₁' : inputs₁.toList = inputs₁'
-      generalize hinputs₂' : inputs₂.toList = inputs₂'
-      generalize houtputs₁' : outputs₁.toList = outputs₁'
-      generalize houtputs₂' : outputs₂.toList = outputs₂'
-      generalize hinputVals₁' : inputVals₁.toList = inputVals₁'
-      generalize hinputVals₂' : inputVals₂.toList = inputVals₂'
-      generalize houtputVals₁' : outputVals₁.toList = outputVals₁'
-      generalize houtputVals₂' : outputVals₂.toList = outputVals₂'
-      rw [hinputs₁', hinputVals₁', houtputs₁', houtputVals₁'] at hinterp₁
-      rw [hinputs₂', hinputVals₂', houtputs₂', houtputVals₂'] at hinterp₂
-      cases hinterp₁ <;> cases hinterp₂
-      all_goals
-        have := pop_vals_eq_head hinputs₁' hinputs₂' hpop₁ hpop₂
-        simp [hinputVals₁', hinputVals₂'] at this
-        subst this
-      case merge.interp_merge_true.interp_merge_true |
-        merge.interp_merge_false.interp_merge_false =>
-        simp [← houtputs₁'] at houtputs₂'
-        have ⟨h₁, h₂⟩ := Vector.toList_inj_heq houtputs₂'
-        subst h₁; subst h₂
-        simp [← hinputs₁'] at hinputs₂'
-        have := Vector.toList_inj.mp hinputs₂'
-        subst this
-        simp [hpop₁] at hpop₂
-        have ⟨h₁, h₂⟩ := hpop₂
-        subst h₁; subst h₂
-        simp [hinputVals₁'] at hinputVals₂'
-        subst hinputVals₂'
-        simp [← houtputVals₁'] at houtputVals₂'
-        have := Vector.toList_inj.mp houtputVals₂'
-        subst this
-        exact ⟨rfl, rfl⟩
-      all_goals grind only
-    | _ =>
-      have heq_inputs := async_op_interp_det_inputs_except_merge hinterp₁ hinterp₂ (by simp)
-      have := Vector.toList_inj.mp heq_inputs
-      subst this
-      simp [hpop₁] at hpop₂
-      have ⟨h₁, h₂⟩ := hpop₂
-      subst h₁; subst h₂
-      have ⟨h₁, h₂, h₃⟩ := async_op_interp_det_outputs hinterp₁ hinterp₂ rfl rfl
-      have ⟨h₁, h₁'⟩ := Vector.toList_inj_heq h₁
-      subst h₁; subst h₁'
-      replace h₂ := Vector.toList_inj.mp h₂
-      subst h₂
-      subst h₃
-      exact ⟨rfl, rfl⟩
+    have heq_inputs := async_op_interp_det_inputs hinterp₁ hinterp₂
+    have ⟨h₁, h₂⟩ := Vector.toList_inj_heq heq_inputs
+    subst h₁; subst h₂
+    simp [hpop₁] at hpop₂
+    have ⟨h₁, h₂⟩ := hpop₂
+    subst h₁; subst h₂
+    have ⟨h₁, h₂, h₃, h₄⟩ := async_op_interp_det_outputs hinterp₁ hinterp₂ rfl
+    replace ⟨h₂, h₂'⟩ := Vector.toList_inj_heq h₂
+    subst h₂; subst h₂'
+    replace h₃ := Vector.toList_inj.mp h₃
+    subst h₃
+    subst h₄
+    exact ⟨rfl, rfl⟩
 
 theorem Config.IndexedStep.unique_index_alt
   [Arity Op] [DecidableEq χ]
